Head normal form for sn terms defined, new Combined kw

proof/Hnf.v
@@ -36,7 +36,8 @@ Proof.
   destruct y ; simpl in *.
   apply (H0 x0 H1 s).
 Qed.
-  
+
+Unset Printing All.
 Program Fixpoint hnf (x : snterm) { wf x sn_ord } :  { y : term | red x y } :=
   match x with
   | App x y => 
@@ -45,200 +46,68 @@ Program Fixpoint hnf (x : snterm) { wf x sn_ord } :  { y : term | red x y } :=
     | Abs T v => hnf (subst y v)
     | h => App h y
     end
-  | Pi1 x =>
-    let nf := hnf x in
-    match nf with
-    | Pair T u v => hnf u
-    | h => Pi1 h
-    end
-  | Pi2 x =>
-    let nf := hnf x in
-    match nf with
-    | Pair T u v => hnf u
-    | h => Pi2 h
-    end
   | _ => x
   end.
 
-Obligations.
 
-Solve Obligations using simpl ; intros ; rewrite <- Heqx ; auto with coc.
+Solve Obligations using simpl ; intros ; rewrite <- H ; auto with coc.
 
-Obligations.
-Obligation 4. 
-simpl ; intros.
-destruct x ; simpl.
-simpl in Heqx.
-assert(subterm x0 x).
-rewrite <- Heqx ; repeat constructor.
-apply subterm_sn with x ; auto.
+Obligation 1.
+  intros.
+  destruct x ; simpl in * ; auto.
+  apply subterm_sn with x ; auto.
+  rewrite <- H ; auto with coc.
 Qed.
 
-Obligations.
-
-Obligation 5.
-  simpl ; intros.
-  destruct x ; simpl.
-  simpl in Heqx.
+Obligation 2.
+  intros.
   unfold sn_ord ; simpl.
-  apply subterm_ord_norm.
-  rewrite <- Heqx ; repeat constructor.
-Qed.
-
-Ltac destruct_call f :=
-  match goal with
-    | H : ?T |- _  =>
-      match T with
-        context [f ?x] => destruct (f x)
-      end
-  end.
-
-
-
-Obligation 6.
-  destruct x ; simpl ; intros ; rewrite <- Heqx ; auto with coc.
-  destruct_call hnf ; simpl in *.
-  apply red_red_app ; auto with coc.
-  rewrite Heqnf ; auto.
-Qed.
-
-Obligation 7.
-  destruct x ; simpl ; intros ; rewrite <- Heqx ; auto with coc.
-  destruct_call hnf ; simpl in * ;
-  apply red_red_app ; auto with coc ;
-  rewrite Heqnf ; auto.
-Qed.
-
-
-Obligation 8.
-  destruct x ; simpl ; intros. 
-  destruct_call hnf ; simpl in *.
-  
-  
-  apply red_red_app ; auto with coc ;
-  rewrite Heqnf ; auto.
-  
-  
-
-
-rewrite Heqx ; auto with coc.
-Qed.
-
-Obligation 3.
-simpl ; intros.
-
   constructor.
-  auto with coc datatypes.
-auto.
-  apply redn_sn_wf.
+  constructor.
+  destruct x ; simpl in * ; auto with coc.
+  rewrite <- H ; auto with coc.
 Qed.
-
 Require Import Coq.subtac.Utils.
 
 Obligation 3.
-  simpl ; intros until x.
-  destruct x ; simpl.
   intros.
-  rewrite <- Heqx.
-  destruct (hnf ((x0 &?))).
-  simpl in HeqHeq_id0.
-  unfold transp ; simpl.
-  
-
-  applt
-  unfold well_founded.
-  unfold snterm.
-  intros.
-  induction a.
-  unfold sn in p.
-  inversion p.
-
-  apply Acc_intro.
-  intros.
-  unfold redn_sn in H ; simpl in H.
-  inversion p.
-  pose (H0 _ H).
-  
-  destruct y.
-  
-  simpl in a.
-  inversion a.
-
-
-
-Inductive hnf : term -> term -> Prop :=
-  | hnf_beta : forall x, forall T e v, 
-    (hnf x (Abs T e) -> 
-    forall H, hnf (subst v e) H ->
-    hnf (App x v) H) ->
-    
-  | hnf_pi1 :  forall p T x y, 
-    hnf p (Pair T x y) ->
-    forall H, hnf x H -> 
-    hnf (Pi1 p) H
-  | hnf_pi2 :  forall p T x y, hnf p (Pair T x y) ->
-    forall H, hnf y H -> hnf (Pi2 p) H
-  | hnf_other : forall x, ~ (exists y, hnf x y /\ y <> x) -> hnf x x.
-
-Lemma hnf_prod : forall U V, hnf (Prod U V) (Prod U V).
-Proof.
-  intros.
-  apply hnf_other.
-  red ; intros.
-  simpl in H.
-  auto.
+  destruct_call hnf.
+  simpl in *.
+  destruct x ; simpl in *.
+  apply sn_red_sn with (App x0 y).
+  subst x ; auto.
+  apply trans_red_red with (App x1 y) ; auto with coc.
+  subst x1 ; auto with coc.
 Qed.
 
-Lemma hnf_function : forall x y z, hnf x y -> hnf x z -> y = z.
-Proof.
-  induction 1 ; simpl ; intros.
-
-  inversion H1 ; subst ; auto.
-  elim H2.
-  simpl.
-  auto.
-
-  inversion H1 ; subst ; auto.
-  elim H2.
-  simpl.
-  auto.
-
-  inversion H1 ; subst ; auto.
-  elim H2.
-  simpl.
-  auto.
-
-  inversion H0.
-  subst.
-  elim H ; simpl ; auto.
-
-  subst.
-  elim H ; simpl ; auto.
-
-  subst.
-  elim H ; simpl ; auto.
-
-  auto.
+Obligation 4.
+  intros.
+  unfold sn_ord.
+  destruct x ; simpl in *.
+  destruct_call hnf ; simpl in *.
+  subst x x1.
+  apply red_red1_ord_norm with (App (Abs T v) y) ; auto with coc.
 Qed.
 
-Lemma hnf_total : forall x, exists y, hnf x y.
-Proof.
-  induction x.
+Obligation 5.
+  intros.
+  destruct_call hnf ; simpl in *.
+  destruct_call hnf ; simpl in *.
+  destruct x ; simpl in *.
+  apply trans_red_red with (subst y v) ; auto.
+  subst x x2.
+  apply trans_red_red with (App (Abs T v) y) ; auto with coc.
+Qed.
 
-  exists (Srt s) ; apply hnf_other ; simpl ; auto.
+Obligation 6.
+  intros.
+  destruct x ; destruct_call hnf ; simpl in *.
+  subst x x1.
+  auto with coc.
+Qed.
 
-  exists (Ref n) ; apply hnf_other ; simpl ; auto.
+Obligation 8.
+  intros.
+  apply redn_sn_wf.  
+Qed.
 
-  exists (Abs x1 x2) ; apply hnf_other ; simpl ; auto.
-
-  (* App *)
-  induction IHx1.
-  induction x1.
-  exists (Srt s) ; apply hnf_other ; simpl ; auto.
-
-
-
-
-
-
-*)
